Automate compiler-building proofs

src/named/CombinedThm.v
@@ -17,44 +17,6 @@ Require Coq.derive.Derive.
 
 
 
-(*TODO: put in right place*)
-
-Import SumboolNotations.
-
-Definition case_eq_dec (r1 r2 : compiler_case) : {r1 = r2} + {~ r1 = r2}.
-  refine(match r1, r2 with
-         | sort_case args t, sort_case args' t' =>
-           SB! (list_eq_dec string_dec args args') SB&
-           (sort_eq_dec t t')
-         | term_case args t, term_case args' t' =>
-           SB! (list_eq_dec string_dec args args') SB&
-           (term_eq_dec t t')
-         | _,_ => _
-         end); autorewrite with utils lang_core; try intuition fail.
-  all: right.
-  all: intros; basic_core_crush.
-Defined.
-
-Definition compute_incl_compiler (l1 l2 : compiler) :=
-  if incl_dec (pair_eq_dec string_dec case_eq_dec) l1 l2 then true else false.
-
-Lemma use_compute_incl_compiler l1 l2
-  : compute_incl_compiler l1 l2 = true -> incl l1 l2.
-Proof.
-  unfold compute_incl_compiler.
-  destruct (incl_dec _ l1 l2); easy.
-Qed.
-
-Ltac solve_incl := 
-  solve [auto with utils
-        | apply use_compute_incl_compiler; vm_compute; reflexivity
-        | apply use_compute_incl_lang; vm_compute; reflexivity].
-
-Ltac use_preserving_hint :=
-  eapply elab_preserving_compiler_embed;
-  [eapply elab_preserving_compiler_monotonicity;[shelve| | shelve |..];
-   [ eauto with elab_pfs| solve_incl|apply use_compute_all_fresh; vm_compute; reflexivity]
-  | solve_incl].
 
 (*TODO: put these hints with their subjects*)
 Hint Resolve cps_preserving : elab_pfs.
@@ -62,11 +24,6 @@ Hint Resolve Ectx_cps_preserving : elab_pfs.
 Hint Resolve fix_cps_preserving : elab_pfs.
 
 Hint Resolve ElabCompilers.elab_preserving_compiler_nil : auto_elab.
-
-
-(*
-TODO: these proofs should be fully automated
- *)
 
 
 (*TODO: add let*)
@@ -85,81 +42,9 @@ Lemma full_cps_compiler_preserving
       (fix_cps++ cps ++ heap_ctx_cps ++ Ectx_cps++ heap_cps++heap_id++cps_subst++[])
       (SimpleVFix.fix_lang++SimpleVSTLC.stlc++ heap_ctx++ eval_ctx++heap_ops++(unit_lang ++ heap ++ nat_exp ++ nat_lang)++(exp_subst ++ value_subst)++[]).
 Proof.
-  eapply elab_compiler_implies_preserving.
-  repeat eapply elab_compiler_prefix_implies_elab; eauto with elab_pfs auto_elab.
-  {
-    eapply elab_preserving_compiler_embed.
-    eapply cps_subst_preserving.
-    solve_incl.
-  }
-  {
-    eapply elab_preserving_compiler_embed.
-    eapply cps_preserving.
-    solve_incl.
-  }
-  {
-    eapply elab_preserving_compiler_embed.
-    eapply heap_cps_preserving.
-    solve_incl.
-  }
-  {
-    eapply elab_preserving_compiler_embed.
-    eapply elab_preserving_compiler_monotonicity.
-    2:eapply Ectx_cps_preserving.
-    change (cps_subst) with (cps_subst++[]).
-    eapply elab_compiler_prefix_implies_elab.
-    constructor.
-    eapply cps_subst_preserving.
-    rewrite <-?app_assoc; solve[prove_from_known_elabs].
-    solve_incl.
-    apply use_compute_all_fresh; vm_compute; reflexivity.
-    solve_incl.
-  }
-  {
-    eapply elab_preserving_compiler_embed.
-    eapply heap_ctx_cps_preserving.
-    solve_incl.
-  }
-  {
-    eapply elab_preserving_compiler_embed.
-    eapply elab_preserving_compiler_monotonicity.
-    2: eapply SimpleVCPS.cps_preserving.
-    change (cps_subst) with (cps_subst++[]).
-    eapply elab_compiler_prefix_implies_elab.
-    constructor.
-    eapply elab_preserving_compiler_embed.
-    eapply cps_subst_preserving.
-    solve_incl.
-    rewrite <-?app_assoc; solve[prove_from_known_elabs].
-    solve_incl.
-    apply use_compute_all_fresh; vm_compute; reflexivity.
-    solve_incl.
-  }
-  {
-    eapply elab_preserving_compiler_embed.
-    eapply elab_preserving_compiler_monotonicity.
-    2: eapply fix_cps_preserving.
-    {
-      eapply elab_compiler_prefix_implies_elab.
-      {
-        change (cps_subst) with (cps_subst++[]).
-        eapply elab_compiler_prefix_implies_elab.
-        constructor.
-        eapply elab_preserving_compiler_embed.
-        eapply cps_subst_preserving.
-        solve_incl.
-      }
-      {
-        eapply elab_preserving_compiler_embed.
-        apply SimpleVCPS.cps_preserving.
-        solve_incl.
-      }
-    }
-    rewrite <-?app_assoc; solve[prove_from_known_elabs].
-    solve_incl.
-    apply use_compute_all_fresh; vm_compute; reflexivity.
-    solve_incl.
-  }
+
+  build_compiler.
+ 
 Qed.
 
 
@@ -173,78 +58,7 @@ Lemma full_cc_compiler_preserving
                         (fix_cps_lang++heap_cps_ops++(unit_lang ++ heap ++ nat_exp ++ nat_lang)
                             ++cps_lang++cps_prod_lang++(block_subst ++ value_subst)++[]).
 Proof.
-  eapply elab_compiler_implies_preserving.
-  repeat eapply elab_compiler_prefix_implies_elab; eauto with elab_pfs auto_elab.
-  {
-    eapply elab_preserving_compiler_embed.
-    eapply subst_cc_preserving.
-    solve_incl.
-  }
-  {
-    eapply elab_preserving_compiler_embed.
-    eapply prod_cc_preserving.
-    solve_incl.
-  }
-  {
-    eapply elab_preserving_compiler_embed.
-    eapply cc_preserving.
-    solve_incl.
-  }
-  {
-    eapply elab_preserving_compiler_monotonicity.
-    2:eapply elab_preserving_compiler_embed.
-    2:eapply heap_id'_preserving.
-    change (subst_cc) with (subst_cc++[]).
-    eapply elab_compiler_prefix_implies_elab.
-    constructor.
-    eapply elab_preserving_compiler_embed.
-    eapply subst_cc_preserving.
-    rewrite <-?app_assoc; solve[prove_from_known_elabs].
-    solve_incl.
-    rewrite <-?app_assoc; solve[prove_from_known_elabs].
-    solve_incl.
-    apply use_compute_all_fresh; vm_compute; reflexivity.
-  }
-  {
-    eapply elab_preserving_compiler_monotonicity.
-    2:eapply elab_preserving_compiler_embed.
-    2:eapply heap_cc_preserving.
-    change (subst_cc) with (subst_cc++[]).
-    eapply elab_compiler_prefix_implies_elab.
-    eapply elab_compiler_prefix_implies_elab.
-    constructor.
-    eapply elab_preserving_compiler_embed.
-    eapply subst_cc_preserving.
-    solve_incl.
-    eapply elab_preserving_compiler_embed.
-    eapply heap_id'_preserving.
-    solve_incl.
-    solve_incl.
-    rewrite <-?app_assoc; solve[prove_from_known_elabs].
-    rewrite <-?app_assoc; solve[prove_from_known_elabs].
-    apply use_compute_all_fresh; vm_compute; reflexivity.
-  }
-  {
-    eapply elab_preserving_compiler_monotonicity.
-    2:eapply elab_preserving_compiler_embed.
-    2:eapply fix_cc_preserving.
-    change (subst_cc) with (subst_cc++[]).
-    repeat eapply elab_compiler_prefix_implies_elab.
-    constructor.
-    eapply elab_preserving_compiler_embed.
-    eapply subst_cc_preserving.
-    solve_incl.
-    eapply elab_preserving_compiler_embed.
-    eapply prod_cc_preserving.
-    solve_incl.
-    eapply elab_preserving_compiler_embed.
-    eapply cc_preserving.
-    solve_incl.    
-    solve_incl.
-    rewrite <-?app_assoc; solve[prove_from_known_elabs].
-    rewrite <-?app_assoc; solve[prove_from_known_elabs].
-    apply use_compute_all_fresh; vm_compute; reflexivity.
-  }
+  build_compiler.
 Qed.
 
 
